add free 8/n: WIP checking ptr validity
deallocate_slab in sight...

src/Slots2.fst
@@ -261,7 +261,103 @@ module US = FStar.SizeT
 // with an additional condition on the offset,
 // then it means it is a valid pointer that *could* be allocated
 // proper alignment means also one can recover the pos of the slot within the slab
+
+#push-options "--z3rlimit 30 --fuel 0 --ifuel 0"
+//TODO: check for spec
 let deallocate_slot_aux0
+  (size_class: sc)
+  (arr: array U8.t{A.length arr = U32.v page_size})
+  (ptr: array U8.t)
+  : Pure bool
+  (requires
+    same_base_array arr ptr /\
+    US.v (ptrdiff (A.ptr_of ptr) (A.ptr_of arr)) < U32.v page_size
+  )
+  (ensures
+    fun r ->
+    r == (US.v (ptrdiff (A.ptr_of ptr) (A.ptr_of arr)) % (U32.v size_class) = 0)
+  )
+  =
+  let diff = ptrdiff (A.ptr_of ptr) (A.ptr_of arr) in
+  assume (US.fits_u32);
+  let size_class_sz = US.uint32_to_sizet size_class in
+  assert (US.v size_class_sz == U32.v size_class);
+  let rem = US.rem diff size_class_sz in
+  assert (US.v rem = US.v diff % U32.v size_class);
+  let r = rem = 0sz in
+  assert (r == (US.v diff % U32.v size_class = 0));
+  r
+
+let slot_array_offset_lemma (size_class: sc) (arr: array U8.t) (pos: U32.t)
+  : Lemma
+  (requires
+    U32.v pos < U32.v (nb_slots size_class) /\
+    A.length arr = U32.v page_size)
+  (ensures
+    U32.v (U32.mul pos size_class)
+    ==
+    A.offset (A.ptr_of (slot_array size_class arr pos)) - A.offset (A.ptr_of arr)
+  )
+  =
+  let ptr = A.ptr_of arr in
+  let shift = U32.mul pos size_class in
+  nb_slots_correct size_class pos;
+  assert (U32.v shift <= U32.v page_size);
+  assert_norm (U32.v shift <= FI.max_int U16.n);
+  assert (U32.v shift <= FI.max_int U16.n);
+  let shift_size_t = STU.small_uint32_to_sizet shift in
+  assert (US.v shift_size_t < A.length arr);
+  let ptr_shifted = A.ptr_shift ptr shift_size_t in
+  assert (ptr_shifted == A.ptr_of (slot_array size_class arr pos));
+  ()
+
+let deallocate_slot_aux1
+  (size_class: sc)
+  (arr: array U8.t{A.length arr = U32.v page_size})
+  (ptr: array U8.t)
+  : Lemma
+  (requires
+    same_base_array arr ptr /\
+    US.v (ptrdiff (A.ptr_of ptr) (A.ptr_of arr)) < U32.v page_size /\
+    US.v (ptrdiff (A.ptr_of ptr) (A.ptr_of arr)) % (U32.v size_class) == 0
+  )
+  (ensures (
+    let diff = ptrdiff (A.ptr_of ptr) (A.ptr_of arr) in
+    let pos = US.v diff / U32.v size_class in
+    pos < U32.v (nb_slots size_class) /\
+    ptr == slot_array size_class arr (U32.uint_to_t pos)
+  ))
+  =
+  let diff = ptrdiff (A.ptr_of ptr) (A.ptr_of arr) in
+  assume (US.fits_u32);
+  let size_class_sz = US.uint32_to_sizet size_class in
+  assert (US.v size_class_sz == U32.v size_class);
+  let pos = US.div diff size_class_sz in
+  let rem = US.rem diff size_class_sz in
+  assume (US.v rem = US.v pos % U32.v size_class);
+  assume (US.v rem == 0);
+  assert (diff = US.mul size_class_sz pos);
+  assume (U32.v (U32.uint_to_t (US.v pos)) < U32.v (nb_slots size_class));
+  slot_array_offset_lemma size_class arr (U32.uint_to_t (US.v pos));
+
+  let ptr' = slot_array size_class arr (U32.uint_to_t (US.v pos)) in
+  assert (A.offset (A.ptr_of ptr) == A.offset (A.ptr_of ptr'));
+  A.ptr_base_offset_inj (A.ptr_of ptr) (A.ptr_of ptr');
+  assert (A.ptr_of ptr == A.ptr_of ptr');
+  // CAUTION: discuss with Aymeric, metaproperty
+  assume (A.length ptr == U32.v size_class);
+  assert (ptr == ptr')
+
+let temp (b: bool)
+  : SteelT unit
+  (if b then emp else emp)
+  (fun _ -> if b then emp else emp)
+  =
+  return ()
+
+(*)
+//TODO: check for spec
+let deallocate_slot_aux1
   (size_class: sc)
   (md: slab_metadata)
   (md_as_seq: G.erased (Seq.lseq U64.t 4))
@@ -270,26 +366,28 @@ let deallocate_slot_aux0
   : Steel bool
   (
     A.varray md `star`
-    A.varray ptr `star`
-    starseq
-      #(pos:U32.t{U32.v pos < U32.v (nb_slots size_class)})
-      #(option (Seq.lseq U8.t (U32.v size_class)))
-      (slab_vprop_aux_f size_class md_as_seq arr)
-      (slab_vprop_aux_f_lemma size_class md_as_seq arr)
-      (SeqUtils.init_u32_refined (U32.v (nb_slots size_class)))
+    A.varray ptr
+//    starseq
+//      #(pos:U32.t{U32.v pos < U32.v (nb_slots size_class)})
+//      #(option (Seq.lseq U8.t (U32.v size_class)))
+//      (slab_vprop_aux_f size_class md_as_seq arr)
+//      (slab_vprop_aux_f_lemma size_class md_as_seq arr)
+//      (SeqUtils.init_u32_refined (U32.v (nb_slots size_class)))
   )
   (fun _ ->
     A.varray md `star`
-    A.varray ptr `star`
-    starseq
-      #(pos:U32.t{U32.v pos < U32.v (nb_slots size_class)})
-      #(option (Seq.lseq U8.t (U32.v size_class)))
-      (slab_vprop_aux_f size_class md_as_seq arr)
-      (slab_vprop_aux_f_lemma size_class md_as_seq arr)
-      (SeqUtils.init_u32_refined (U32.v (nb_slots size_class)))
+    A.varray ptr
+//    starseq
+//      #(pos:U32.t{U32.v pos < U32.v (nb_slots size_class)})
+//      #(option (Seq.lseq U8.t (U32.v size_class)))
+//      (slab_vprop_aux_f size_class md_as_seq arr)
+//      (slab_vprop_aux_f_lemma size_class md_as_seq arr)
+//      (SeqUtils.init_u32_refined (U32.v (nb_slots size_class)))
   )
   (requires fun h0 ->
     same_base_array arr ptr /\
+    US.v (ptrdiff (A.ptr_of ptr) (A.ptr_of arr)) < U32.v page_size /\
+    US.v (ptrdiff (A.ptr_of ptr) (A.ptr_of arr)) % (U32.v size_class) /\
     A.asel md h0 == G.reveal md_as_seq
   )
   (ensures fun _ _ _ -> True)
@@ -300,6 +398,8 @@ let deallocate_slot_aux0
   let rem = US.rem diff size_class_sz in
   let r = rem = 0sz in
   return r
+
+
 
 (*)
 - [ok] ptrdiff
